set/cunningham: 1.2. substitution in equivalences
one step to proove that any variable in any logical equivalence (law) could be replaced by any expression

set/cunningham/1_intro/2_Logic.v
@@ -3,11 +3,38 @@ Require Import Setoid.
 Require Import Morphisms.
 From Stdlib Require Import Classical.
 From Stdlib Require Import List. Import ListNotations.
-Require Import Bool.
-Require Import Nat.
+From Stdlib Require Import Bool.
+From Stdlib Require Import Nat.
+From Stdlib Require Import Strings.Ascii.
 From Stdlib Require Import Strings.String.
 
 Open Scope bool_scope.
+
+(** some aux facts *)
+
+Theorem negb_sym (a b: bool): negb a = b <-> a = negb b.
+Proof. destruct a, b; simpl; intuition. Qed.  
+
+Theorem contraposition (A B: Prop): (A -> B) -> (~ B -> ~ A).
+Proof.
+  intros HAB HnB HA. apply HnB, HAB, HA.
+Qed.
+
+Theorem not_in_cons {X: Type} (y x: X) (xs: list X):
+  ~ In y (x :: xs) -> x <> y /\ ~ In y xs.
+Proof.
+  intro H. simpl in H. split.
+  - intro eq. apply H. left. exact eq.
+  - intro Hc. apply H. right. exact Hc.
+Qed.
+
+Theorem not_in_app {X: Type} (x: X) (xs ys: list X):
+  ~ In x (xs ++ ys) -> ~ In x xs /\ ~ In x ys.
+Proof.
+  intro H. split; intro C; apply H; apply in_or_app.
+  - left. exact C.
+  - right. exact C.
+Qed.
 
 (** Propositions and Logical Connectives *)
 (* boolean statement *)
@@ -57,6 +84,7 @@ Unset Printing Notations.
 Check <{ ~(P & Q | P) <-> ~P | F }>.
 Set Printing Notations.
 
+(** String Map *)
 Definition SMap (X: Type) := string -> X.
 Definition SMap_default {X: Type} (x: X): SMap X := fun _ => x.
 Definition SMap_update {X: Type} (m: SMap X) (k: string) (x: X): SMap X :=
@@ -66,9 +94,83 @@ Notation "'_' '!->' x" := (SMap_default x) (at level 100, right associativity).
 Notation "k '!->' x ';' m" :=
   (SMap_update m k x) (at level 100, k constr, right associativity).
 
+Theorem SMap_update_eq {X: Type} (k: string) (x: X) (m: SMap X):
+  (k !-> x; m) k = x.
+Proof. unfold SMap_update. rewrite eqb_refl. reflexivity. Qed.
+
+Theorem SMap_update_neq {X: Type} (k x: string) (v: X) (m: SMap X):
+  k <> x -> (k !-> v; m) x = m x.
+Proof.
+  unfold SMap_update. intro neq.
+  apply eqb_neq in neq. rewrite eqb_sym. rewrite neq. reflexivity.
+Qed.
+
+(* map pointwise equality *)
+Definition EqM {X: Type} (m n: SMap X) := forall x, m x = n x.
+Notation "m == n" := (EqM m n) (at level 70, no associativity).
+
+Instance EqM_refl {X: Type}: Reflexive (@EqM X).
+Proof. unfold Reflexive, EqM. reflexivity. Qed.
+
+Instance EqM_sym {X: Type}: Symmetric (@EqM X).
+Proof. unfold Symmetric, EqM. auto. Qed.
+
+Instance EqM_trans {X: Type}: Transitive (@EqM X).
+Proof.
+  unfold Transitive, EqM.
+  intros m n p H1 H2 x. rewrite H1, H2. reflexivity.
+Qed.
+
+Instance EqM_equiv {X: Type}: Equivalence (@EqM X).
+Proof.
+  split. 
+  - apply EqM_refl.
+  - apply EqM_sym.
+  - apply EqM_trans.
+Qed.
+
+Theorem SMap_update_same {X: Type} (m: SMap X) (k: string):
+  (k !-> m k; m) == m.
+Proof.
+  intro x. unfold SMap_update. destruct (eqb_spec x k) as [eq|neq].
+  - subst x. reflexivity.
+  - reflexivity.
+Qed.
+
+Theorem SMap_same_update {X: Type} (m: SMap X) (k: string) (u v: X):
+  (k !-> v; k !-> u; m) == (k !-> v; m).
+Proof.
+  intro x. unfold SMap_update.
+  destruct (eqb_spec x k) as [eq|neq]; reflexivity.
+Qed.
+
+Instance EqM_update_proper {X: Type}:
+  Proper (EqM ==> eq ==> eq ==> EqM) (@SMap_update X).
+Proof.
+  unfold Proper, respectful.
+  intros m n eq_mn u v eq_uv x y eq_xy k. subst y u.
+  unfold SMap_update. destruct (eqb_spec k v) as [eq_kv|neq_kv].
+  - reflexivity.
+  - apply eq_mn.
+Qed.
+
+Theorem SMap_update_inj {X: Type} (k: string) (v: X) (m n: SMap X):
+  m == n -> (k !-> v; m) == (k !-> v; n).
+Proof. intro eq. rewrite eq. reflexivity. Qed.
+
+Theorem SMap_update_reorder {X: Type} (k1 k2: string) (v1 v2: X) (m: SMap X):
+  k1 <> k2 -> (k1 !-> v1; k2 !-> v2; m) == (k2 !-> v2; k1 !-> v1; m).
+Proof.
+  intros neq x. unfold SMap_update.
+  destruct (eqb_spec x k1) as [eq1|neq1], (eqb_spec x k2) as [eq2|neq2];
+    try reflexivity.
+  contradict eq2. subst x. exact neq.
+Qed.
+
 Definition PQ_vals: list (SMap bool) :=
   map (fun '(p, q) => (P !-> p; Q !-> q; _ !-> F)) (list_prod bvals bvals).
 
+(** eval *)
 Fixpoint eval (m: SMap bool) (s: St): bool :=
   match s with
   | StConst b => b
@@ -97,6 +199,22 @@ Compute map (fun m => (m P, m Q, eval m pr1)) PQ_vals.
 
 Example pr1_is_p (m: SMap bool): eval m pr1 = eval m P.
 Proof. simpl. destruct (m P), (m Q); reflexivity. Qed.
+
+Instance EqM_eval_proper: Proper (EqM ==> eq ==> eq) eval.
+Proof.
+  unfold Proper, respectful.
+  intros x y H s t eq. subst t.
+  generalize dependent y.
+  generalize dependent x.
+  induction s; intros x y H; simpl.
+  - reflexivity.
+  - apply H.
+  - rewrite (IHs x y) by exact H. reflexivity.
+  - rewrite (IHs1 x y), (IHs2 x y) by exact H. reflexivity.
+  - rewrite (IHs1 x y), (IHs2 x y) by exact H. reflexivity.
+  - rewrite (IHs1 x y), (IHs2 x y) by exact H. reflexivity.
+  - rewrite (IHs1 x y), (IHs2 x y) by exact H. reflexivity.
+Qed.
 
 Definition ConstB (b: bool) (s: St): Prop := forall m, eval m s = b.
 
@@ -193,6 +311,12 @@ Proof.
   destruct (eval m p), (eval m q); reflexivity.
 Qed.
 
+Theorem DMLB1': <{ ~(P | Q) }> <=> <{ ~P & ~Q }>.
+Proof.
+  unfold EqB. intro m. simpl.
+  destruct (m P), (m Q); reflexivity.
+Qed.
+
 Theorem DML1 (P Q: Prop): ~(P \/ Q) <-> ~P /\ ~Q.
 Proof.
   split; intro H.
@@ -229,3 +353,453 @@ Proof.
   discriminate C.
 Qed.
 
+(* Propositional Logic Laws *)
+
+Section StSubstitution.
+
+(* substitute all instances of [StVar k] in [p] by [r] *)
+Fixpoint St_subst (k: string) (r p: St): St :=
+  match p with
+  | StConst _ as x => x
+  | StVar name as x => if name =? k then r else x
+  | StNot x => StNot (St_subst k r x)
+  | StAnd x y => StAnd (St_subst k r x) (St_subst k r y)
+  | StOr x y => StOr (St_subst k r x) (St_subst k r y)
+  | StImpl x y => StImpl (St_subst k r x) (St_subst k r y)
+  | StIff x y => StIff (St_subst k r x) (St_subst k r y)
+  end.
+
+Theorem all_eval_andb_true_iff (s t: St):
+  (forall m, eval m s && eval m t = true) <->
+    (forall m, eval m s = true) /\ (forall m, eval m t = true).
+Proof.
+  split; intro H.
+  - split; intro m.
+    + pose (H m) as Hm. apply andb_true_iff in Hm as [H1 H2]. exact H1.
+    + pose (H m) as Hm. apply andb_true_iff in Hm as [H1 H2]. exact H2.
+  - intro m. destruct H as [H1 H2].
+    rewrite H1, H2. reflexivity.
+Qed.
+
+Theorem all_eval_andb_false_iff (s t: St):
+  (forall m, eval m s && eval m t = false) <->
+    (forall m, eval m s = false \/ eval m t = false).
+Proof.
+  split; intros H m; pose (H m) as Hm.
+  - apply andb_false_iff in Hm.
+    destruct Hm as [H1 | H2]; auto.
+  - apply andb_false_iff. exact Hm.
+Qed.
+
+Theorem St_subst_prop (k: string) (s r: St) (m: SMap bool):
+  eval m (St_subst k r s) = eval (k !-> eval m r; m) s.
+Proof.
+  generalize dependent m.
+  induction s as [b | v | s IH | s1 IH1 s2 IH2
+                 | s1 IH1 s2 IH2 | s1 IH1 s2 IH2 | s1 IH1 s2 IH2];
+    intro m.
+  - (* s = StConst b *) reflexivity.
+  - (* s = StVar v *) simpl. destruct (v =? k) eqn:eq.
+    + (* v = k *) apply eqb_eq in eq. rewrite eq, SMap_update_eq. reflexivity.
+    + (* v <> k *) unfold SMap_update. rewrite eq. reflexivity.
+  - (* s = StNot *) simpl. pose (IH m) as H. rewrite H. reflexivity.
+  - (* s = StAnd *) simpl. rewrite IH1, IH2. reflexivity.
+  - (* s = StOr *) simpl. rewrite IH1, IH2. reflexivity.
+  - (* s = StImpl *) simpl. rewrite IH1, IH2. reflexivity.
+  - (* s = StIff *) simpl. rewrite IH1, IH2. reflexivity.
+Qed.
+
+Theorem St_subst_in_const (b: bool) (k: string) (s r: St):
+  (forall m, eval m s = b) -> (forall n, eval n (St_subst k r s) = b).
+Proof.
+  intros H n.
+  pose (St_subst_prop k s r n) as E.
+  rewrite E. apply H.
+Qed.
+
+Instance EqB_subst_proper (k: string) (r: St): Proper (EqB ==> EqB) (St_subst k r).
+Proof.
+  unfold Proper, respectful, EqB. intros p q H m.
+  rewrite !St_subst_prop. rewrite H. reflexivity.
+Qed.
+
+Theorem EqB_subst (k: string) (r p q: St):
+  p <=> q -> St_subst k r p <=> St_subst k r q.
+Proof.
+  intro H. rewrite H. reflexivity.
+Qed.
+
+Theorem eval_eq (m n: SMap bool) (s t: St):
+  s <=> t -> m == n -> eval m s = eval n t.
+Proof.
+  intros eq_st eq_ev.
+  rewrite eq_ev. apply eq_st.
+Qed.
+
+(** rename to avoid collisins *)
+(* fresh_str *)
+Fixpoint longest_str (x: string) (xs: list string): string :=
+  match xs with
+  | [] => x
+  | y :: ys => if Nat.ltb (length x) (length y)
+             then longest_str y ys
+             else longest_str x ys
+  end.
+
+Lemma longest_str_head (x: string) (xs: list string):
+  length x <= length (longest_str x xs).
+Proof.
+  generalize dependent x.
+  induction xs as [| y xs IH]; intro x.
+  { simpl. apply le_n. }
+  simpl. destruct (length x <? length y)%nat eqn:H.
+  - apply PeanoNat.Nat.ltb_lt in H. apply PeanoNat.Nat.lt_le_incl.
+    apply PeanoNat.Nat.lt_le_trans with (length y).
+    { exact H. } apply IH.
+  - apply IH.
+Qed.
+
+Lemma longest_str_tail (x y: string) (xs: list string):
+  In y xs -> length y <= length (longest_str x xs).
+Proof.
+  generalize dependent y.
+  generalize dependent x.
+  induction xs as [| z xs IH]; intros x y H. { inversion H. }
+  simpl in H. destruct H as [H | H].
+  - subst z. simpl. destruct (length x <? length y)%nat eqn:H1.
+    { apply longest_str_head. }
+    apply PeanoNat.Nat.ltb_ge in H1.
+    apply PeanoNat.Nat.le_trans with (length x). { exact H1. }
+    apply longest_str_head.
+  - simpl. destruct (length x <? length z)%nat eqn:H1.
+    + apply IH. apply H.
+    + apply IH. apply H.
+Qed.
+
+Theorem longest_str_prop (x: string) (xs: list string):
+  forall y: string, In y (x :: xs) -> length y <= length (longest_str x xs).
+Proof.
+  intros y [H | H].
+  - subst y. apply longest_str_head.
+  - apply longest_str_tail. apply H.
+Qed.
+
+Definition fresh_str (xs: list string): string :=
+  match xs with
+  | [] => ""
+  | x :: xs => String "x"%char (longest_str x xs)
+  end.
+
+Theorem fresh_str_longer (x: string) (xs: list string):
+  let f := fresh_str (x :: xs)
+  in length (longest_str x xs) < length f.
+Proof. simpl. apply PeanoNat.Nat.lt_succ_diag_r. Qed.
+
+Theorem fresh_str_longest (xs: list string):
+  forall y: string, In y xs -> length y < length (fresh_str xs).
+Proof.
+  intros y H. destruct xs as [| x xs]. { inversion H. }
+  apply PeanoNat.Nat.le_lt_trans with (length (longest_str x xs)).
+  - apply longest_str_prop. apply H.
+  - apply fresh_str_longer.
+Qed.
+
+Theorem fresh_str_fresh (xs: list string): ~ In (fresh_str xs) xs.
+Proof.
+  intro H. apply fresh_str_longest in H.
+  apply (PeanoNat.Nat.lt_irrefl _ H).
+Qed.
+
+Theorem fresh_str_cons_fresh_head (x: string) (xs: list string):
+  x <> fresh_str (x :: xs).
+Proof.
+  pose (fresh_str_longer x xs) as H1. intro H.
+  rewrite <- H in H1. simpl in H1.
+  assert (length x <= length (longest_str x xs)) as H2.
+  { apply longest_str_prop. apply in_eq. }
+  assert (length x < length x) as C.
+  { apply PeanoNat.Nat.le_lt_trans with (length (longest_str x xs)).
+    - exact H2.
+    - exact H1. }
+  apply (PeanoNat.Nat.lt_irrefl (length x)). exact C.
+Qed.  
+
+Theorem fresh_str_cons_fresh_tail (x: string) (xs: list string):
+  ~ In (fresh_str (x :: xs)) xs.
+Proof.
+  intro H. apply fresh_str_fresh with (x :: xs).
+  remember (fresh_str (x :: xs)) as f eqn:eq.
+  apply in_cons. exact H.
+Qed.
+
+Theorem fresh_str_cons_prop (f x: string) (xs: list string):
+  f = fresh_str (x :: xs) -> x <> f /\ ~ In f xs.
+Proof.
+  intro H. subst f. split.
+  - apply fresh_str_cons_fresh_head.
+  - apply fresh_str_cons_fresh_tail.
+Qed.
+
+Theorem fresh_str_app_l_fresh (xs ys: list string):
+  ~ In (fresh_str (xs ++ ys)) xs.
+Proof.
+  induction xs as [| x xs IH]. { auto. }
+  simpl. intros [H | H].
+  { apply (fresh_str_cons_fresh_head x (xs ++ ys) H). }
+  apply (fresh_str_cons_fresh_tail x (xs ++ ys)). simpl.
+  apply in_or_app. left. exact H.
+Qed.
+
+Theorem fresh_str_app_r_fresh (xs ys: list string):
+  ~ In (fresh_str (xs ++ ys)) ys.
+Proof.
+  induction xs as [| x xs IH]. { simpl. apply fresh_str_fresh. }
+  simpl. intros H. apply (fresh_str_cons_fresh_tail x (xs ++ ys)). simpl.
+  apply in_or_app. right. exact H.
+Qed.
+
+Theorem fresh_str_app_prop (f: string) (xs ys: list string):
+  f = fresh_str (xs ++ ys) -> ~ In f xs /\ ~ In f ys.
+Proof.
+  intro H. subst f. split.
+  - apply fresh_str_app_l_fresh.
+  - apply fresh_str_app_r_fresh.
+Qed.
+
+(* list vars *)
+Fixpoint list_vars (s: St): list string :=
+  match s with
+  | StConst b => []
+  | StVar v => [v]
+  | StNot x => list_vars x
+  | StAnd x y => list_vars x ++ list_vars y
+  | StOr x y => list_vars x ++ list_vars y
+  | StImpl x y => list_vars x ++ list_vars y
+  | StIff x y => list_vars x ++ list_vars y
+  end.
+
+Fixpoint StIn (x: string) (s: St): Prop :=
+  match s with
+  | StConst b => False
+  | StVar v => x = v
+  | StNot t => StIn x t
+  | StAnd t u => StIn x t \/ StIn x u
+  | StOr t u => StIn x t \/ StIn x u
+  | StImpl t u => StIn x t \/ StIn x u
+  | StIff t u => StIn x t \/ StIn x u
+  end.
+
+Theorem StIn_prop (x: string) (s: St): StIn x s <-> In x (list_vars s).
+Proof.
+  induction s; simpl; intuition.
+  - apply in_app_or in H3 as [H3 | H3]; intuition.
+  - apply in_app_or in H3 as [H3 | H3]; intuition.
+  - apply in_app_or in H3 as [H3 | H3]; intuition.
+  - apply in_app_or in H3 as [H3 | H3]; intuition.
+Qed.
+
+Theorem fresh_str_not_In_St (s: St): ~ StIn (fresh_str (list_vars s)) s.
+Proof. rewrite StIn_prop. apply fresh_str_fresh. Qed.
+
+Theorem eval_fresh (m: SMap bool) (k: string) (v: bool) (s: St):
+  ~ StIn k s -> eval (k !-> v; m) s = eval m s.
+Proof.
+  induction s; simpl; intro Hf.
+  - reflexivity.
+  - apply eqb_neq in Hf. unfold SMap_update.
+    rewrite eqb_sym, Hf. reflexivity.
+  - apply IHs in Hf as IH. rewrite IH. reflexivity.
+  - apply DML1 in Hf as [H1 H2]. rewrite (IHs1 H1), (IHs2 H2). reflexivity.
+  - apply DML1 in Hf as [H1 H2]. rewrite (IHs1 H1), (IHs2 H2). reflexivity.
+  - apply DML1 in Hf as [H1 H2]. rewrite (IHs1 H1), (IHs2 H2). reflexivity.
+  - apply DML1 in Hf as [H1 H2]. rewrite (IHs1 H1), (IHs2 H2). reflexivity.
+Qed.
+
+(* rename all StVar's with name = u to v *)
+Definition St_rename (u v: string) (s: St) := St_subst u (StVar v) s.
+
+Theorem St_rename_id (k: string) (s: St): St_rename k k s = s.
+Proof.
+  induction s; unfold St_rename in * |- *; simpl.
+  - reflexivity.
+  - destruct (eqb_spec name k) as [eq|neq].
+    + simpl. subst k. reflexivity.
+    + simpl. reflexivity.
+  - rewrite IHs. reflexivity.
+  - rewrite IHs1, IHs2; try assumption. reflexivity.
+  - rewrite IHs1, IHs2; try assumption. reflexivity.
+  - rewrite IHs1, IHs2; try assumption. reflexivity.
+  - rewrite IHs1, IHs2; try assumption. reflexivity.
+Qed.
+
+Theorem St_rename_equiv_back (u v: string) (s: St) (m: SMap bool):
+  eval m (St_rename u v s) = eval (u !-> m v; m) s.
+Proof. unfold St_rename. apply St_subst_prop. Qed.
+
+Theorem St_rename_involutive (u v: string) (s: St):
+  ~ StIn v s -> s = St_rename v u (St_rename u v s).
+Proof.
+  unfold St_rename. induction s; simpl; intro Hn.
+  - reflexivity.
+  - destruct (eqb_spec name u) as [eq|neq].
+    + simpl. rewrite eqb_refl. subst u. reflexivity.
+    + simpl. apply eqb_neq in Hn. rewrite eqb_sym. rewrite Hn. reflexivity.
+  - rewrite <- IHs. { reflexivity. } exact Hn.
+  - apply not_or_and in Hn. destruct Hn as [H1 H2].
+    rewrite <- IHs1, <- IHs2; try assumption. reflexivity.
+  - apply not_or_and in Hn. destruct Hn as [H1 H2].
+    rewrite <- IHs1, <- IHs2; try assumption. reflexivity.
+  - apply not_or_and in Hn. destruct Hn as [H1 H2].
+    rewrite <- IHs1, <- IHs2; try assumption. reflexivity.
+  - apply not_or_and in Hn. destruct Hn as [H1 H2].
+    rewrite <- IHs1, <- IHs2; try assumption. reflexivity.
+Qed.
+
+Theorem St_rename_equiv (u v: string) (s: St) (m: SMap bool):
+  ~ StIn v s -> eval m s = eval (v !-> m u; m) (St_rename u v s).
+Proof.
+  intro Hn. rewrite (St_rename_involutive u v s Hn) at 1.
+  apply St_rename_equiv_back.
+Qed.  
+
+Theorem St_rename_fresh (m: SMap bool) (k f: string) (s: St) (v: bool):
+  ~ StIn f s -> eval m (St_rename k f s) = eval (k !-> v; m) (St_rename k f s).
+Proof.
+  intro Hf. unfold St_rename. rewrite !St_subst_prop.
+  simpl. destruct (eqb_spec k f) as [eq|neq].
+  - subst f. rewrite SMap_update_eq.
+    rewrite !(eval_fresh _ k _ s Hf). reflexivity.
+  - rewrite (SMap_update_neq k f v m neq).
+    rewrite SMap_same_update. reflexivity.
+Qed.
+
+Theorem St_subst_fresh (f: string) (r s: St): ~ StIn f s -> St_subst f r s = s.
+Proof.
+  induction s; simpl; intro nin; try rewrite IHs1, IHs2; auto.
+  - destruct (eqb_spec name f) as [eq|neq].
+    + subst name. contradiction nin. reflexivity.
+    + reflexivity.
+  - rewrite IHs; auto.
+Qed.
+
+Theorem StIn_rename (f k: string) (s: St):
+  StIn k (St_rename k f s) -> StIn k s /\ f = k.
+Proof.
+  unfold St_rename. induction s; simpl; intro H; intuition;
+    destruct (eqb_spec name k) as [eq|neq]; simpl in H.
+  - subst name f. reflexivity.
+  - subst name. contradict neq. reflexivity.
+  - subst name f. reflexivity.
+  - subst name. contradict neq. reflexivity.
+Qed.
+
+Theorem St_not_in_fresh_rename (f k: string) (s: St):
+  ~ StIn f s -> ~ StIn k (St_rename k f s).
+Proof.
+  intros C H. apply StIn_rename in H as [H eq].
+  subst f. apply C, H.
+Qed.
+
+Theorem St_subst_after_fresh_rename (f k: string) (r s: St):
+  ~ StIn f s -> St_subst k r (St_rename k f s) = St_rename k f s.
+Proof.
+  intro H. apply St_subst_fresh. apply St_not_in_fresh_rename, H.
+Qed.
+
+Theorem St_subst_with_fresh_rename (f k: string) (r s: St):
+  ~ StIn f s -> St_subst f r (St_rename k f s) = St_subst k r s.
+Proof.
+  unfold St_rename. induction s; simpl; intro H;
+    try rewrite IHs1, IHs2; auto.
+  - destruct (eqb_spec name k) as [eq|neq]; simpl.
+    + rewrite eqb_refl. reflexivity.
+    + apply eqb_neq in H. rewrite eqb_sym. rewrite H. reflexivity.
+  - rewrite (IHs H). reflexivity.
+Qed.
+
+Theorem St_subst_fresh_reorder (k1 k2: string) (r1 r2 s: St):
+  k1 <> k2 -> ~ StIn k1 r2 -> ~ StIn k2 r1
+  -> St_subst k1 r1 (St_subst k2 r2 s) = St_subst k2 r2 (St_subst k1 r1 s).
+Proof.
+  induction s; simpl; intros neq H1 H2.
+  - reflexivity.
+  - destruct (eqb_spec name k1) as [eq1 | neq1];
+      destruct (eqb_spec name k2) as [eq2 | neq2]; simpl.
+    + subst k2 name. contradict neq. reflexivity.
+    + subst name. rewrite eqb_refl.
+      rewrite St_subst_fresh; [ reflexivity | exact H2 ].
+    + subst name. rewrite eqb_refl.
+      rewrite St_subst_fresh; [ reflexivity | exact H1 ].
+    + apply eqb_neq in neq1. apply eqb_neq in neq2.
+      rewrite neq1, neq2. reflexivity.
+  - rewrite IHs; auto.
+  - rewrite IHs1, IHs2; auto.
+  - rewrite IHs1, IHs2; auto.
+  - rewrite IHs1, IHs2; auto.
+  - rewrite IHs1, IHs2; auto.
+Qed.
+
+Definition St_subst2 (k1: string) (r1: St) (k2: string) (r2 s: St): St :=
+  let f := fresh_str (k1 :: k2 :: (list_vars r1) ++ (list_vars r2) ++ (list_vars s)) in
+  let r1' := St_rename k2 f r1 in
+  let s1 := St_subst k1 r1' s in
+  let s2 := St_subst k2 r2 s1
+  in St_rename f k2 s2.
+
+Instance EqB_subst2_proper (k1: string) (r1: St) (k2: string) (r2: St):
+  Proper (EqB ==> EqB) (St_subst2 k1 r1 k2 r2).
+Proof.
+  unfold Proper, respectful, EqB, St_subst2. intros p q H m.
+  remember (fresh_str (k1 :: k2 :: list_vars r1 ++ list_vars r2 ++ list_vars p))
+    as fp eqn:eq_fp.
+  remember (fresh_str (k1 :: k2 :: list_vars r1 ++ list_vars r2 ++ list_vars q))
+    as fq eqn:eq_fq.
+  rewrite !St_rename_equiv_back. rewrite !St_subst_prop.
+  remember (fp !-> m k2; m) as mp eqn:eq_mp.
+  remember (fq !-> m k2; m) as mq eqn:eq_mq.
+  pose (fresh_str_cons_prop fp k1 _ eq_fp) as Hp.
+  destruct Hp as [neq_fp_k1 Hp]. apply not_in_cons in Hp as [neq_fp_k2 Hp].
+  apply not_in_app in Hp as [Hpr1 Hp]. apply not_in_app in Hp as [Hpr2 Hp].
+  pose (fresh_str_cons_prop fq k1 _ eq_fq) as Hq.
+  destruct Hq as [neq_fq_k1 Hq]. apply not_in_cons in Hq as [neq_fq_k2 Hq].
+  apply not_in_app in Hq as [Hqr1 Hq]. apply not_in_app in Hq as [Hqr2 Hq].
+  rewrite <- StIn_prop in Hpr1, Hpr2, Hp, Hqr1, Hqr2, Hq.
+  rewrite <- !St_rename_fresh by assumption.
+  rewrite eq_mp at 3. rewrite <- St_rename_equiv by assumption.
+  rewrite eq_mq at 3. rewrite <- St_rename_equiv by assumption.
+  subst mp mq.
+  rewrite (eval_fresh m fp), (eval_fresh m fq) by assumption.
+  rewrite (SMap_update_reorder k2 fp), (SMap_update_reorder k1 fp) by assumption.
+  rewrite (eval_fresh _ fp) by assumption.
+  rewrite (SMap_update_reorder k2 fq), (SMap_update_reorder k1 fq) by assumption.
+  rewrite (eval_fresh _ fq) by assumption.
+  rewrite H. reflexivity.
+Qed.
+
+Theorem EqB_subst2 (k1: string) (r1: St) (k2: string) (r2 p q: St):
+  p <=> q -> St_subst2 k1 r1 k2 r2 p <=> St_subst2 k1 r1 k2 r2 q.
+Proof.
+  intro H. rewrite H. reflexivity.
+Qed.
+
+Theorem DMLB1_ex (p q: St): <{ ~(p | q) }> <=> <{ ~p & ~q }>.
+Proof.
+  pose DMLB1' as H.
+  apply (EqB_subst2 P p Q q) in H. unfold St_subst2 in H. simpl in H.
+  remember (String "x" (longest_str P (list_vars p ++ list_vars q ++ [P; Q])))
+    as f eqn:eq_f.
+  assert (f = fresh_str (P :: Q :: list_vars p ++ list_vars q ++ [P; Q])) as eq_f'.
+  { simpl. exact eq_f. }
+  pose (fresh_str_cons_prop f _ _ eq_f') as nin. destruct nin as [neq_fp nin].
+  apply not_in_cons in nin as [neq_fq nin].
+  apply not_in_app in nin as [nin_p nin]. apply not_in_app in nin as [nin_q _].
+  rewrite <- StIn_prop in nin_p, nin_q.
+  rewrite St_subst_after_fresh_rename in H by assumption.
+  unfold St_rename in H. simpl in H. fold (St_rename Q f p) in H.
+  rewrite St_subst_with_fresh_rename in H by assumption.
+  fold (St_rename Q Q p) in H.
+  rewrite St_rename_id in H.
+  rewrite St_subst_fresh in H by assumption. exact H.
+Qed.
+
+End StSubstitution.
